wip: correctness of the merkle root calculation with padding

examples/low-level/merkletree/MerkleTree.High.fst
@@ -44,7 +44,6 @@ val seq_map_create:
 	[SMTPat (seq_map f (S.create len ia))]
 let rec seq_map_create #a #b f len ia =
   S.lemma_eq_intro (seq_map f (S.create len ia)) (S.create len (f ia))
-  // S.lemma_eq_elim (seq_map f (S.create len ia)) (S.create len (f ia))
 
 val seq_map_append:
   #a:Type -> #b:Type -> f:(a -> b) -> 
@@ -56,12 +55,29 @@ let rec seq_map_append #a #b f s1 s2 =
   S.lemma_eq_elim (seq_map f (S.append s1 s2)) 
 		  (S.append (seq_map f s1) (seq_map f s2))
 
+val seq_map_slice:
+  #a:Type -> #b:Type -> f:(a -> b) -> 
+  s:S.seq a -> i:nat -> j:nat{i <= j && j <= length s} ->
+  Lemma (seq_map f (S.slice s i j) == S.slice (seq_map f s) i j)
+	[SMTPat (seq_map f (S.slice s i j)); 
+	SMTPat (S.slice (seq_map f s) i j)]
+let seq_map_slice #a #b f s i j =
+  S.lemma_eq_elim (seq_map f (S.slice s i j))
+		  (S.slice (seq_map f s) i j)
+
 val lemma_split_append:
   #a:Type -> s1:S.seq a -> s2:S.seq a ->
   Lemma (S.split (S.append s1 s2) (S.length s1) == (s1, s2))
 let lemma_split_append #a s1 s2 =
   S.lemma_eq_elim (fst (S.split (S.append s1 s2) (S.length s1))) s1;
   S.lemma_eq_elim (snd (S.split (S.append s1 s2) (S.length s1))) s2
+
+val seq_create_one_cons:
+  #a:eqtype -> ia:a -> 
+  Lemma (S.create 1 ia = S.cons ia S.empty)
+	[SMTPat (S.create 1 ia); SMTPat (S.cons ia S.empty)]
+let seq_create_one_cons #a ia =
+  S.lemma_eq_elim (S.create 1 ia) (S.cons ia S.empty)
 
 /// Power of two (TODO: use a bit vector; division is expensive)
 
@@ -92,6 +108,16 @@ val pow2_floor:
 let rec pow2_floor n =
   if n = 1 then 0 else 1 + pow2_floor (n / 2)
 
+val pow2_ceil:
+  n:nat{n > 0} -> 
+  GTot (p:nat{
+    if n = 1 then p = 0
+    else (p > 0 && pow2 (p - 1) < n && n <= pow2 p)})
+let rec pow2_ceil n =
+  if n = 1 then 0
+  else if n % 2 = 0 then 1 + pow2_ceil (n / 2)
+  else 1 + pow2_ceil ((n + 1) / 2)
+
 val pow2_floor_pow2:
   p:nat -> 
   Lemma (pow2_floor (pow2 p) = p)
@@ -99,6 +125,15 @@ val pow2_floor_pow2:
 let rec pow2_floor_pow2 p =
   if p = 0 then ()
   else pow2_floor_pow2 (p - 1)
+
+val pow2_ceil_pow2:
+  p:nat -> 
+  Lemma (pow2_ceil (pow2 p) = p)
+	[SMTPat (pow2_ceil (pow2 p))]
+let rec pow2_ceil_pow2 p =
+  if p = 0 then ()
+  else (assert (pow2 p / 2 = pow2 (p - 1));
+       pow2_ceil_pow2 (p - 1))
 
 val pow2_floor_is_pow2:
   n:nat ->
@@ -108,6 +143,15 @@ val pow2_floor_is_pow2:
 let rec pow2_floor_is_pow2 n =
   if n = 1 then ()
   else pow2_floor_is_pow2 (n / 2)
+
+val pow2_ceil_is_pow2:
+  n:nat ->
+  Lemma (requires (is_pow2 n))
+	(ensures (n = pow2 (pow2_ceil n)))
+	[SMTPat (is_pow2 n)]
+let rec pow2_ceil_is_pow2 n =
+  if n = 1 then ()
+  else pow2_ceil_is_pow2 (n / 2)
 
 val pow2_interval_unique:
   n:nat -> p1:nat -> p2:nat ->
@@ -139,6 +183,12 @@ val pow2_floor_pow2_pow2:
 let pow2_floor_pow2_pow2 p q =
   Math.Lemmas.pow2_lt_compat p q;
   pow2_floor_pow2_less p (pow2 q)
+
+val not_pow2_floor_ceil:
+  n:nat{n > 0 && not (is_pow2 n)} ->
+  Lemma (pow2_floor n + 1 = pow2_ceil n)
+let not_pow2_floor_ceil n =
+  admit ()
 
 /// Invariants between internal roots and values
 
@@ -189,7 +239,6 @@ val iroots_of_hashes_pow2_same:
 	S.create 1 (hash_from_hashes 
 	  (S.index (iroots_of_hashes hs1) 0)
 	  (S.index (iroots_of_hashes hs2) 0)))
-
 let iroots_of_hashes_pow2_same hs1 hs2 =
   S.lemma_eq_elim (S.cons (merkle_root_of_pow2 (S.append hs1 hs2)) S.empty)
   		  (S.create 1 (merkle_root_of_pow2 (S.append hs1 hs2)));
@@ -248,8 +297,6 @@ noeq type merkle_tree =
 
 val create_merkle_tree: unit -> merkle_tree
 let create_merkle_tree _ = 
-  S.lemma_eq_elim (iroots_of (S.create 1 elem_init))
-  		  (S.create 1 (hash_from_elem elem_init));
   MT (S.create 1 elem_init) (S.create 1 (hash_from_elem elem_init))
 
 /// Insertion
@@ -275,14 +322,19 @@ val iroots_of_head:
   Lemma (iroots_of (S.slice vs 0 (pow2 (pow2_floor (S.length vs)))) =
 	S.create 1 (S.head (iroots_of vs)))
 let iroots_of_head vs =
-  admit ()
+  let hs = seq_map hash_from_elem vs in
+  let n_floor = pow2 (pow2_floor (S.length vs)) in
+  assert (S.head (iroots_of vs) = merkle_root_of_pow2 (S.slice hs 0 n_floor))
 
 val iroots_of_tail:
   vs:elem_seq{S.length vs > 0} ->
   Lemma (iroots_of (S.slice vs (pow2 (pow2_floor (S.length vs))) (S.length vs)) =
 	S.tail (iroots_of vs))
 let iroots_of_tail vs =
-  admit ()
+  let hs = seq_map hash_from_elem vs in
+  let n_floor = pow2 (pow2_floor (S.length vs)) in
+  S.lemma_tl (merkle_root_of_pow2 (S.slice hs 0 n_floor))
+	     (iroots_of_hashes (S.slice hs n_floor (S.length hs)))
 
 val insert_iroots:
   vs:elem_seq{S.length vs > 0} ->
@@ -290,6 +342,7 @@ val insert_iroots:
   nv:elem ->
   GTot (iirs:hash_seq{iroots_of (insert_values vs nv) = iirs})
        (decreases (S.length irs))
+#set-options "--z3rlimit 10"
 let rec insert_iroots vs irs nv =
   if S.length vs = 0
   then (S.create 1 (hash_from_elem nv))
@@ -316,45 +369,72 @@ let insert mt e =
 
 /// Getting the Merkle root
 
-val padding_to_pow2:
-  nelts:nat{nelts > 0} -> GTot (sz:nat{
-    if nelts = 1 then sz = 0
-    else sz > 0 && pow2 (sz - 1) < nelts && nelts <= pow2 sz})
-let rec padding_to_pow2 nelts =
-  if nelts = 1 then 0
-  else if nelts % 2 = 0 then 1 + padding_to_pow2 (nelts / 2)
-  else 1 + padding_to_pow2 ((nelts + 1) / 2)
-
 val pad_hashes_pow2:
   vs:hash_seq{S.length vs > 0} -> 
   GTot (pvs:hash_seq{
-    S.length pvs = pow2 (padding_to_pow2 (S.length vs)) && 
+    S.length pvs = pow2 (pow2_ceil (S.length vs)) && 
     S.slice pvs 0 (S.length vs) = vs})
 let pad_hashes_pow2 vs =
-  let pad = S.create (pow2 (padding_to_pow2 (S.length vs)) - S.length vs) hash_init in
+  let pad = S.create (pow2 (pow2_ceil (S.length vs)) - S.length vs) hash_init in
   S.append_slices vs pad;
   S.append vs pad
+
+val pad_hashes_pow2_pow2:
+  vs:hash_seq{is_pow2 (S.length vs)} ->
+  Lemma (pad_hashes_pow2 vs = vs)
+let pad_hashes_pow2_pow2 vs = ()
 
 val merkle_root_of_hashes: vs:hash_seq{S.length vs > 0} -> GTot hash
 let merkle_root_of_hashes vs =
   merkle_root_of_pow2 (pad_hashes_pow2 vs)
 
-val merkle_root_of_iroots':
-  acc:hash -> irs:hash_seq -> GTot hash (decreases (S.length irs))
-let rec merkle_root_of_iroots' acc irs =
-  if S.length irs = 0 then acc
-  else merkle_root_of_iroots'
-       (hash_from_hashes (S.index irs (S.length irs - 1)) acc)
-       (S.tail irs)
-
-val merkle_root_of_iroots: irs:hash_seq -> GTot hash
+val merkle_root_of_iroots: 
+  irs:hash_seq{S.length irs > 0} -> 
+  GTot hash (decreases (S.length irs))
 let rec merkle_root_of_iroots irs =
-  merkle_root_of_iroots' hash_init irs
+  if S.length irs = 1 then S.index irs 0
+  else hash_from_hashes (S.head irs) (merkle_root_of_iroots (S.tail irs))
+
+val merkle_root_of_iroots_ok_hashes:
+  vs:hash_seq{S.length vs > 0} ->
+  irs:hash_seq{iroots_of_hashes vs = irs} ->
+  Lemma (merkle_root_of_iroots irs = merkle_root_of_hashes vs)
+#set-options "--z3rlimit 20"
+let rec merkle_root_of_iroots_ok_hashes vs irs =
+  if is_pow2 (S.length vs)
+  then (assert (irs = S.cons (merkle_root_of_pow2 vs) S.empty);
+       hash_init_idem (merkle_root_of_pow2 vs))
+  else (assert (S.length irs > 1);
+       assert (merkle_root_of_iroots irs =
+	      hash_from_hashes (S.head irs) (merkle_root_of_iroots (S.tail irs)));
+       let pvs = pad_hashes_pow2 vs in
+       assert (merkle_root_of_hashes vs = merkle_root_of_pow2 pvs);
+       assert (S.length pvs > 1);
+       // assert (merkle_root_of_pow2 pvs =
+       // 	      hash_from_hashes 
+       // 	      	(merkle_root_of_pow2 (S.slice pvs 0 (S.length pvs / 2)))
+       // 	      	(merkle_root_of_pow2 (S.slice pvs (S.length pvs / 2) (S.length pvs))));
+
+       // not_pow2_floor_ceil (S.length vs);
+       // Math.Lemmas.pow2_double_mult (pow2_floor (S.length vs));
+       // assert (2 * pow2 (pow2_floor (S.length vs)) = pow2 (pow2_ceil (S.length vs)));
+       // assert (pow2 (pow2_floor (S.length vs)) = pow2 (pow2_ceil (S.length vs)) / 2);
+       // assert (S.head irs = merkle_root_of_pow2 (S.slice vs 0 (pow2 (pow2_floor (S.length vs)))));
+       // !!! assume (S.head irs = merkle_root_of_pow2 (S.slice pvs 0 (S.length pvs / 2)));
+
+       // assert (merkle_root_of_iroots (S.tail irs) =
+       // 	      merkle_root_of_hashes (S.slice vs (pow2 (pow2_floor (length vs))) (length vs)));
+       // TODO HERE: should prove that any length of padding will not change the merkle root value.
+       // !!! assume (merkle_root_of_iroots (S.tail irs) =
+       // 	      merkle_root_of_pow2 (S.slice pvs (S.length pvs / 2) (S.length pvs)));
+       admit ())
 
 val merkle_root_of_iroots_ok:
   mt:merkle_tree ->
   Lemma (merkle_root_of_iroots (MT?.iroots mt) =
 	merkle_root_of_hashes (seq_map hash_from_elem (MT?.values mt)))
 let merkle_root_of_iroots_ok mt =
-  admit ()
+  merkle_root_of_iroots_ok_hashes
+    (seq_map hash_from_elem (MT?.values mt))
+    (MT?.iroots mt)
 
